src/Basics.v
@@ -61,3 +61,49 @@ Proof.
       constructor. apply (H 0); simpl; lia. eapply IHl1; auto. intros. apply (H (S i)).
       simpl. lia.
 Qed.
+
+Theorem biforall_length :
+  forall {T1 T2 : Type} (es : list T1) (es' : list T2) P, list_biforall P es es' -> length es = length es'.
+Proof.
+  intros. induction H; auto. simpl. auto.
+Qed.
+
+Lemma biforall_impl : forall {T1 T2} (l1 : list T1) (l2 : list T2) (P Q : T1 -> T2 -> Prop),
+  (forall x y, P x y -> Q x y) ->
+  list_biforall P l1 l2 -> list_biforall Q l1 l2.
+Proof.
+  induction l1; intros; inversion H0; constructor; subst.
+  now apply H.
+  eapply IHl1; eauto.
+Qed.
+
+Lemma biforall_app : forall {T1 T2} (l1 l1' : list T1) (l2 l2' : list T2) P,
+  list_biforall P l1 l2 -> list_biforall P l1' l2'
+->
+  list_biforall P (l1 ++ l1') (l2 ++ l2').
+Proof.
+  induction l1; intros.
+  * inversion H. auto.
+  * inversion H. subst. do 2 rewrite <- app_comm_cons. constructor; auto. 
+Qed.
+
+Lemma biforall_map :
+  forall {T1 T2 T1' T2'} l l' f1 f2 (P : T1 -> T2 -> Prop) (Q : T1' -> T2' -> Prop), list_biforall P l l' ->
+  (forall x y, P x y -> Q (f1 x) (f2 y))
+->
+  list_biforall Q (map f1 l) (map f2 l').
+Proof.
+  induction l; intros; inversion H; simpl; constructor; subst.
+  * inversion H. subst. apply H0; auto.
+  * eapply IHl; eauto.
+Qed.
+
+Lemma biforall_forall_refl : forall {T} (l: list T) P, list_biforall P l l -> Forall (fun x => P x x) l.
+Proof.
+  induction l; constructor; inversion H; subst; auto.
+Qed.
+
+Lemma forall_biforall_refl : forall {T} (l: list T) P, Forall (fun x => P x x) l -> list_biforall P l l.
+Proof.
+  induction l; constructor; inversion H; subst; auto.
+Qed.
